test/lean/localvar.lean
@@ -1,0 +1,407 @@
+import Clightdefs
+open CC
+
+namespace Localvar
+
+namespace Info
+  def version : String := "3.17"
+  def build_number : String := ""
+  def build_tag : String := ""
+  def build_branch : String := ""
+  def arch : String := "aarch64"
+  def model : String := "default"
+  def abi : String := "apple"
+  def bitsize : Nat := 64
+  def big_endian : Bool := false
+  def source_file : String := "localvar.c"
+  def normalized : Bool := true
+end Info
+
+def ___builtin_annot : Ident := identOfString "__builtin_annot"
+def ___builtin_annot_intval : Ident := identOfString "__builtin_annot_intval"
+def ___builtin_bswap : Ident := identOfString "__builtin_bswap"
+def ___builtin_bswap16 : Ident := identOfString "__builtin_bswap16"
+def ___builtin_bswap32 : Ident := identOfString "__builtin_bswap32"
+def ___builtin_bswap64 : Ident := identOfString "__builtin_bswap64"
+def ___builtin_cls : Ident := identOfString "__builtin_cls"
+def ___builtin_clsl : Ident := identOfString "__builtin_clsl"
+def ___builtin_clsll : Ident := identOfString "__builtin_clsll"
+def ___builtin_clz : Ident := identOfString "__builtin_clz"
+def ___builtin_clzl : Ident := identOfString "__builtin_clzl"
+def ___builtin_clzll : Ident := identOfString "__builtin_clzll"
+def ___builtin_ctz : Ident := identOfString "__builtin_ctz"
+def ___builtin_ctzl : Ident := identOfString "__builtin_ctzl"
+def ___builtin_ctzll : Ident := identOfString "__builtin_ctzll"
+def ___builtin_debug : Ident := identOfString "__builtin_debug"
+def ___builtin_expect : Ident := identOfString "__builtin_expect"
+def ___builtin_fabs : Ident := identOfString "__builtin_fabs"
+def ___builtin_fabsf : Ident := identOfString "__builtin_fabsf"
+def ___builtin_fmadd : Ident := identOfString "__builtin_fmadd"
+def ___builtin_fmax : Ident := identOfString "__builtin_fmax"
+def ___builtin_fmin : Ident := identOfString "__builtin_fmin"
+def ___builtin_fmsub : Ident := identOfString "__builtin_fmsub"
+def ___builtin_fnmadd : Ident := identOfString "__builtin_fnmadd"
+def ___builtin_fnmsub : Ident := identOfString "__builtin_fnmsub"
+def ___builtin_fsqrt : Ident := identOfString "__builtin_fsqrt"
+def ___builtin_membar : Ident := identOfString "__builtin_membar"
+def ___builtin_memcpy_aligned : Ident := identOfString "__builtin_memcpy_aligned"
+def ___builtin_sel : Ident := identOfString "__builtin_sel"
+def ___builtin_sqrt : Ident := identOfString "__builtin_sqrt"
+def ___builtin_unreachable : Ident := identOfString "__builtin_unreachable"
+def ___builtin_va_arg : Ident := identOfString "__builtin_va_arg"
+def ___builtin_va_copy : Ident := identOfString "__builtin_va_copy"
+def ___builtin_va_end : Ident := identOfString "__builtin_va_end"
+def ___builtin_va_start : Ident := identOfString "__builtin_va_start"
+def ___compcert_i64_dtos : Ident := identOfString "__compcert_i64_dtos"
+def ___compcert_i64_dtou : Ident := identOfString "__compcert_i64_dtou"
+def ___compcert_i64_sar : Ident := identOfString "__compcert_i64_sar"
+def ___compcert_i64_sdiv : Ident := identOfString "__compcert_i64_sdiv"
+def ___compcert_i64_shl : Ident := identOfString "__compcert_i64_shl"
+def ___compcert_i64_shr : Ident := identOfString "__compcert_i64_shr"
+def ___compcert_i64_smod : Ident := identOfString "__compcert_i64_smod"
+def ___compcert_i64_smulh : Ident := identOfString "__compcert_i64_smulh"
+def ___compcert_i64_stod : Ident := identOfString "__compcert_i64_stod"
+def ___compcert_i64_stof : Ident := identOfString "__compcert_i64_stof"
+def ___compcert_i64_udiv : Ident := identOfString "__compcert_i64_udiv"
+def ___compcert_i64_umod : Ident := identOfString "__compcert_i64_umod"
+def ___compcert_i64_umulh : Ident := identOfString "__compcert_i64_umulh"
+def ___compcert_i64_utod : Ident := identOfString "__compcert_i64_utod"
+def ___compcert_i64_utof : Ident := identOfString "__compcert_i64_utof"
+def ___compcert_va_composite : Ident := identOfString "__compcert_va_composite"
+def ___compcert_va_float64 : Ident := identOfString "__compcert_va_float64"
+def ___compcert_va_int32 : Ident := identOfString "__compcert_va_int32"
+def ___compcert_va_int64 : Ident := identOfString "__compcert_va_int64"
+def _a : Ident := identOfString "a"
+def _b : Ident := identOfString "b"
+def _main : Ident := identOfString "main"
+def _s : Ident := identOfString "s"
+def _sink : Ident := identOfString "sink"
+def _st : Ident := identOfString "st"
+def _use_local : Ident := identOfString "use_local"
+def _x : Ident := identOfString "x"
+def _t'1 : Ident := (Positive.ofNat 128)
+
+def f_use_local : Function := {
+  fn_return := tuint,
+  fn_callconv := cc_default,
+  fn_params := [(_x, tuint)],
+  fn_vars := [(_s, (Ty.Tstruct _st noattr))],
+  fn_temps := [(_t'1, tuint)],
+  fn_body :=
+(Stmt.Ssequence
+  (Stmt.Sassign (Expr.Efield (Expr.Evar _s (Ty.Tstruct _st noattr)) _a tuint)
+    (Expr.Etempvar _x tuint))
+  (Stmt.Ssequence
+    (Stmt.Sassign
+      (Expr.Efield (Expr.Evar _s (Ty.Tstruct _st noattr)) _b tuint)
+      (Expr.Econst_int (Integers.Int.repr 7) tint))
+    (Stmt.Ssequence
+      (Stmt.Scall (some _t'1)
+        (Expr.Evar _sink (Ty.Tfunction [(tptr (Ty.Tstruct _st noattr))] tuint
+                           cc_default))
+        [(Expr.Eaddrof (Expr.Evar _s (Ty.Tstruct _st noattr))
+           (tptr (Ty.Tstruct _st noattr)))])
+      (Stmt.Sreturn (some (Expr.Etempvar _t'1 tuint))))))
+}
+
+def composites : List CompositeDef :=
+[(CompositeDef.Composite _st SU.Struct
+   [(Member.Member_plain _a tuint), (Member.Member_plain _b tuint)]
+   noattr)]
+
+def global_definitions : List (Ident × GlobDef FunDef Ty) :=
+[(___compcert_va_int32,
+   GlobDef.Gfun (FunDef.External (ExtFun.EF_runtime "__compcert_va_int32"
+                                   (mksignature [XType.Xptr] XType.Xint
+                                     cc_default)) [(tptr tvoid)] tuint
+     cc_default)),
+ (___compcert_va_int64,
+   GlobDef.Gfun (FunDef.External (ExtFun.EF_runtime "__compcert_va_int64"
+                                   (mksignature [XType.Xptr] XType.Xlong
+                                     cc_default)) [(tptr tvoid)] tulong
+     cc_default)),
+ (___compcert_va_float64,
+   GlobDef.Gfun (FunDef.External (ExtFun.EF_runtime "__compcert_va_float64"
+                                   (mksignature [XType.Xptr] XType.Xfloat
+                                     cc_default)) [(tptr tvoid)] tdouble
+     cc_default)),
+ (___compcert_va_composite,
+   GlobDef.Gfun (FunDef.External (ExtFun.EF_runtime "__compcert_va_composite"
+                                   (mksignature [XType.Xptr, XType.Xlong]
+                                     XType.Xptr cc_default))
+     [(tptr tvoid), tulong] (tptr tvoid) cc_default)),
+ (___compcert_i64_dtos,
+   GlobDef.Gfun (FunDef.External (ExtFun.EF_runtime "__compcert_i64_dtos"
+                                   (mksignature [XType.Xfloat] XType.Xlong
+                                     cc_default)) [tdouble] tlong
+     cc_default)),
+ (___compcert_i64_dtou,
+   GlobDef.Gfun (FunDef.External (ExtFun.EF_runtime "__compcert_i64_dtou"
+                                   (mksignature [XType.Xfloat] XType.Xlong
+                                     cc_default)) [tdouble] tulong
+     cc_default)),
+ (___compcert_i64_stod,
+   GlobDef.Gfun (FunDef.External (ExtFun.EF_runtime "__compcert_i64_stod"
+                                   (mksignature [XType.Xlong] XType.Xfloat
+                                     cc_default)) [tlong] tdouble
+     cc_default)),
+ (___compcert_i64_utod,
+   GlobDef.Gfun (FunDef.External (ExtFun.EF_runtime "__compcert_i64_utod"
+                                   (mksignature [XType.Xlong] XType.Xfloat
+                                     cc_default)) [tulong] tdouble
+     cc_default)),
+ (___compcert_i64_stof,
+   GlobDef.Gfun (FunDef.External (ExtFun.EF_runtime "__compcert_i64_stof"
+                                   (mksignature [XType.Xlong] XType.Xsingle
+                                     cc_default)) [tlong] tfloat cc_default)),
+ (___compcert_i64_utof,
+   GlobDef.Gfun (FunDef.External (ExtFun.EF_runtime "__compcert_i64_utof"
+                                   (mksignature [XType.Xlong] XType.Xsingle
+                                     cc_default)) [tulong] tfloat
+     cc_default)),
+ (___compcert_i64_sdiv,
+   GlobDef.Gfun (FunDef.External (ExtFun.EF_runtime "__compcert_i64_sdiv"
+                                   (mksignature [XType.Xlong, XType.Xlong]
+                                     XType.Xlong cc_default)) [tlong, tlong]
+     tlong cc_default)),
+ (___compcert_i64_udiv,
+   GlobDef.Gfun (FunDef.External (ExtFun.EF_runtime "__compcert_i64_udiv"
+                                   (mksignature [XType.Xlong, XType.Xlong]
+                                     XType.Xlong cc_default))
+     [tulong, tulong] tulong cc_default)),
+ (___compcert_i64_smod,
+   GlobDef.Gfun (FunDef.External (ExtFun.EF_runtime "__compcert_i64_smod"
+                                   (mksignature [XType.Xlong, XType.Xlong]
+                                     XType.Xlong cc_default)) [tlong, tlong]
+     tlong cc_default)),
+ (___compcert_i64_umod,
+   GlobDef.Gfun (FunDef.External (ExtFun.EF_runtime "__compcert_i64_umod"
+                                   (mksignature [XType.Xlong, XType.Xlong]
+                                     XType.Xlong cc_default))
+     [tulong, tulong] tulong cc_default)),
+ (___compcert_i64_shl,
+   GlobDef.Gfun (FunDef.External (ExtFun.EF_runtime "__compcert_i64_shl"
+                                   (mksignature [XType.Xlong, XType.Xint]
+                                     XType.Xlong cc_default)) [tlong, tint]
+     tlong cc_default)),
+ (___compcert_i64_shr,
+   GlobDef.Gfun (FunDef.External (ExtFun.EF_runtime "__compcert_i64_shr"
+                                   (mksignature [XType.Xlong, XType.Xint]
+                                     XType.Xlong cc_default)) [tulong, tint]
+     tulong cc_default)),
+ (___compcert_i64_sar,
+   GlobDef.Gfun (FunDef.External (ExtFun.EF_runtime "__compcert_i64_sar"
+                                   (mksignature [XType.Xlong, XType.Xint]
+                                     XType.Xlong cc_default)) [tlong, tint]
+     tlong cc_default)),
+ (___compcert_i64_smulh,
+   GlobDef.Gfun (FunDef.External (ExtFun.EF_runtime "__compcert_i64_smulh"
+                                   (mksignature [XType.Xlong, XType.Xlong]
+                                     XType.Xlong cc_default)) [tlong, tlong]
+     tlong cc_default)),
+ (___compcert_i64_umulh,
+   GlobDef.Gfun (FunDef.External (ExtFun.EF_runtime "__compcert_i64_umulh"
+                                   (mksignature [XType.Xlong, XType.Xlong]
+                                     XType.Xlong cc_default))
+     [tulong, tulong] tulong cc_default)),
+ (___builtin_bswap64,
+   GlobDef.Gfun (FunDef.External (ExtFun.EF_builtin "__builtin_bswap64"
+                                   (mksignature [XType.Xlong] XType.Xlong
+                                     cc_default)) [tulong] tulong
+     cc_default)),
+ (___builtin_bswap,
+   GlobDef.Gfun (FunDef.External (ExtFun.EF_builtin "__builtin_bswap"
+                                   (mksignature [XType.Xint] XType.Xint
+                                     cc_default)) [tuint] tuint cc_default)),
+ (___builtin_bswap32,
+   GlobDef.Gfun (FunDef.External (ExtFun.EF_builtin "__builtin_bswap32"
+                                   (mksignature [XType.Xint] XType.Xint
+                                     cc_default)) [tuint] tuint cc_default)),
+ (___builtin_bswap16,
+   GlobDef.Gfun (FunDef.External (ExtFun.EF_builtin "__builtin_bswap16"
+                                   (mksignature [XType.Xint16unsigned]
+                                     XType.Xint16unsigned cc_default))
+     [tushort] tushort cc_default)),
+ (___builtin_clz,
+   GlobDef.Gfun (FunDef.External (ExtFun.EF_builtin "__builtin_clz"
+                                   (mksignature [XType.Xint] XType.Xint
+                                     cc_default)) [tuint] tint cc_default)),
+ (___builtin_clzl,
+   GlobDef.Gfun (FunDef.External (ExtFun.EF_builtin "__builtin_clzl"
+                                   (mksignature [XType.Xlong] XType.Xint
+                                     cc_default)) [tulong] tint cc_default)),
+ (___builtin_clzll,
+   GlobDef.Gfun (FunDef.External (ExtFun.EF_builtin "__builtin_clzll"
+                                   (mksignature [XType.Xlong] XType.Xint
+                                     cc_default)) [tulong] tint cc_default)),
+ (___builtin_ctz,
+   GlobDef.Gfun (FunDef.External (ExtFun.EF_builtin "__builtin_ctz"
+                                   (mksignature [XType.Xint] XType.Xint
+                                     cc_default)) [tuint] tint cc_default)),
+ (___builtin_ctzl,
+   GlobDef.Gfun (FunDef.External (ExtFun.EF_builtin "__builtin_ctzl"
+                                   (mksignature [XType.Xlong] XType.Xint
+                                     cc_default)) [tulong] tint cc_default)),
+ (___builtin_ctzll,
+   GlobDef.Gfun (FunDef.External (ExtFun.EF_builtin "__builtin_ctzll"
+                                   (mksignature [XType.Xlong] XType.Xint
+                                     cc_default)) [tulong] tint cc_default)),
+ (___builtin_fabs,
+   GlobDef.Gfun (FunDef.External (ExtFun.EF_builtin "__builtin_fabs"
+                                   (mksignature [XType.Xfloat] XType.Xfloat
+                                     cc_default)) [tdouble] tdouble
+     cc_default)),
+ (___builtin_fabsf,
+   GlobDef.Gfun (FunDef.External (ExtFun.EF_builtin "__builtin_fabsf"
+                                   (mksignature [XType.Xsingle] XType.Xsingle
+                                     cc_default)) [tfloat] tfloat
+     cc_default)),
+ (___builtin_fsqrt,
+   GlobDef.Gfun (FunDef.External (ExtFun.EF_builtin "__builtin_fsqrt"
+                                   (mksignature [XType.Xfloat] XType.Xfloat
+                                     cc_default)) [tdouble] tdouble
+     cc_default)),
+ (___builtin_sqrt,
+   GlobDef.Gfun (FunDef.External (ExtFun.EF_builtin "__builtin_sqrt"
+                                   (mksignature [XType.Xfloat] XType.Xfloat
+                                     cc_default)) [tdouble] tdouble
+     cc_default)),
+ (___builtin_memcpy_aligned,
+   GlobDef.Gfun (FunDef.External (ExtFun.EF_builtin "__builtin_memcpy_aligned"
+                                   (mksignature
+                                     [XType.Xptr, XType.Xptr, XType.Xlong,
+                                      XType.Xlong] XType.Xvoid cc_default))
+     [(tptr tvoid), (tptr tvoid), tulong, tulong] tvoid cc_default)),
+ (___builtin_sel,
+   GlobDef.Gfun (FunDef.External (ExtFun.EF_builtin "__builtin_sel"
+                                   (mksignature [XType.Xbool] XType.Xvoid
+                                     { cc_vararg := (some 1), cc_unproto := false, cc_structret := false }))
+     [tbool] tvoid
+     { cc_vararg := (some 1), cc_unproto := false, cc_structret := false })),
+ (___builtin_annot,
+   GlobDef.Gfun (FunDef.External (ExtFun.EF_builtin "__builtin_annot"
+                                   (mksignature [XType.Xptr] XType.Xvoid
+                                     { cc_vararg := (some 1), cc_unproto := false, cc_structret := false }))
+     [(tptr tschar)] tvoid
+     { cc_vararg := (some 1), cc_unproto := false, cc_structret := false })),
+ (___builtin_annot_intval,
+   GlobDef.Gfun (FunDef.External (ExtFun.EF_builtin "__builtin_annot_intval"
+                                   (mksignature [XType.Xptr, XType.Xint]
+                                     XType.Xint cc_default))
+     [(tptr tschar), tint] tint cc_default)),
+ (___builtin_membar,
+   GlobDef.Gfun (FunDef.External (ExtFun.EF_builtin "__builtin_membar"
+                                   (mksignature [] XType.Xvoid cc_default))
+     [] tvoid cc_default)),
+ (___builtin_va_start,
+   GlobDef.Gfun (FunDef.External (ExtFun.EF_builtin "__builtin_va_start"
+                                   (mksignature [XType.Xptr] XType.Xvoid
+                                     cc_default)) [(tptr tvoid)] tvoid
+     cc_default)),
+ (___builtin_va_arg,
+   GlobDef.Gfun (FunDef.External (ExtFun.EF_builtin "__builtin_va_arg"
+                                   (mksignature [XType.Xptr, XType.Xint]
+                                     XType.Xvoid cc_default))
+     [(tptr tvoid), tuint] tvoid cc_default)),
+ (___builtin_va_copy,
+   GlobDef.Gfun (FunDef.External (ExtFun.EF_builtin "__builtin_va_copy"
+                                   (mksignature [XType.Xptr, XType.Xptr]
+                                     XType.Xvoid cc_default))
+     [(tptr tvoid), (tptr tvoid)] tvoid cc_default)),
+ (___builtin_va_end,
+   GlobDef.Gfun (FunDef.External (ExtFun.EF_builtin "__builtin_va_end"
+                                   (mksignature [XType.Xptr] XType.Xvoid
+                                     cc_default)) [(tptr tvoid)] tvoid
+     cc_default)),
+ (___builtin_unreachable,
+   GlobDef.Gfun (FunDef.External (ExtFun.EF_builtin "__builtin_unreachable"
+                                   (mksignature [] XType.Xvoid cc_default))
+     [] tvoid cc_default)),
+ (___builtin_expect,
+   GlobDef.Gfun (FunDef.External (ExtFun.EF_builtin "__builtin_expect"
+                                   (mksignature [XType.Xlong, XType.Xlong]
+                                     XType.Xlong cc_default)) [tlong, tlong]
+     tlong cc_default)),
+ (___builtin_cls,
+   GlobDef.Gfun (FunDef.External (ExtFun.EF_builtin "__builtin_cls"
+                                   (mksignature [XType.Xint] XType.Xint
+                                     cc_default)) [tint] tint cc_default)),
+ (___builtin_clsl,
+   GlobDef.Gfun (FunDef.External (ExtFun.EF_builtin "__builtin_clsl"
+                                   (mksignature [XType.Xlong] XType.Xint
+                                     cc_default)) [tlong] tint cc_default)),
+ (___builtin_clsll,
+   GlobDef.Gfun (FunDef.External (ExtFun.EF_builtin "__builtin_clsll"
+                                   (mksignature [XType.Xlong] XType.Xint
+                                     cc_default)) [tlong] tint cc_default)),
+ (___builtin_fmadd,
+   GlobDef.Gfun (FunDef.External (ExtFun.EF_builtin "__builtin_fmadd"
+                                   (mksignature
+                                     [XType.Xfloat, XType.Xfloat,
+                                      XType.Xfloat] XType.Xfloat cc_default))
+     [tdouble, tdouble, tdouble] tdouble cc_default)),
+ (___builtin_fmsub,
+   GlobDef.Gfun (FunDef.External (ExtFun.EF_builtin "__builtin_fmsub"
+                                   (mksignature
+                                     [XType.Xfloat, XType.Xfloat,
+                                      XType.Xfloat] XType.Xfloat cc_default))
+     [tdouble, tdouble, tdouble] tdouble cc_default)),
+ (___builtin_fnmadd,
+   GlobDef.Gfun (FunDef.External (ExtFun.EF_builtin "__builtin_fnmadd"
+                                   (mksignature
+                                     [XType.Xfloat, XType.Xfloat,
+                                      XType.Xfloat] XType.Xfloat cc_default))
+     [tdouble, tdouble, tdouble] tdouble cc_default)),
+ (___builtin_fnmsub,
+   GlobDef.Gfun (FunDef.External (ExtFun.EF_builtin "__builtin_fnmsub"
+                                   (mksignature
+                                     [XType.Xfloat, XType.Xfloat,
+                                      XType.Xfloat] XType.Xfloat cc_default))
+     [tdouble, tdouble, tdouble] tdouble cc_default)),
+ (___builtin_fmax,
+   GlobDef.Gfun (FunDef.External (ExtFun.EF_builtin "__builtin_fmax"
+                                   (mksignature [XType.Xfloat, XType.Xfloat]
+                                     XType.Xfloat cc_default))
+     [tdouble, tdouble] tdouble cc_default)),
+ (___builtin_fmin,
+   GlobDef.Gfun (FunDef.External (ExtFun.EF_builtin "__builtin_fmin"
+                                   (mksignature [XType.Xfloat, XType.Xfloat]
+                                     XType.Xfloat cc_default))
+     [tdouble, tdouble] tdouble cc_default)),
+ (___builtin_debug,
+   GlobDef.Gfun (FunDef.External (ExtFun.EF_external "__builtin_debug"
+                                   (mksignature [XType.Xint] XType.Xvoid
+                                     { cc_vararg := (some 1), cc_unproto := false, cc_structret := false }))
+     [tint] tvoid
+     { cc_vararg := (some 1), cc_unproto := false, cc_structret := false })),
+ (_sink,
+   GlobDef.Gfun (FunDef.External (ExtFun.EF_external "sink"
+                                   (mksignature [XType.Xptr] XType.Xint
+                                     cc_default))
+     [(tptr (Ty.Tstruct _st noattr))] tuint cc_default)),
+ (_use_local, GlobDef.Gfun (FunDef.Internal f_use_local))]
+
+def public_idents : List Ident :=
+[_use_local, _sink, ___builtin_debug, ___builtin_fmin, ___builtin_fmax,
+ ___builtin_fnmsub, ___builtin_fnmadd, ___builtin_fmsub, ___builtin_fmadd,
+ ___builtin_clsll, ___builtin_clsl, ___builtin_cls, ___builtin_expect,
+ ___builtin_unreachable, ___builtin_va_end, ___builtin_va_copy,
+ ___builtin_va_arg, ___builtin_va_start, ___builtin_membar,
+ ___builtin_annot_intval, ___builtin_annot, ___builtin_sel,
+ ___builtin_memcpy_aligned, ___builtin_sqrt, ___builtin_fsqrt,
+ ___builtin_fabsf, ___builtin_fabs, ___builtin_ctzll, ___builtin_ctzl,
+ ___builtin_ctz, ___builtin_clzll, ___builtin_clzl, ___builtin_clz,
+ ___builtin_bswap16, ___builtin_bswap32, ___builtin_bswap,
+ ___builtin_bswap64, ___compcert_i64_umulh, ___compcert_i64_smulh,
+ ___compcert_i64_sar, ___compcert_i64_shr, ___compcert_i64_shl,
+ ___compcert_i64_umod, ___compcert_i64_smod, ___compcert_i64_udiv,
+ ___compcert_i64_sdiv, ___compcert_i64_utof, ___compcert_i64_stof,
+ ___compcert_i64_utod, ___compcert_i64_stod, ___compcert_i64_dtou,
+ ___compcert_i64_dtos, ___compcert_va_composite, ___compcert_va_float64,
+ ___compcert_va_int64, ___compcert_va_int32]
+
+def prog : Program :=
+  mkprogram composites global_definitions public_idents _main
+
+end Localvar
+
